Compilatore LOOP -> SCORE

MasterThesis/SCORE/Compiler.lean
@@ -1,3 +1,34 @@
 import MasterThesis.SCORE.Language
+import MasterThesis.SCORE.Interpreter
 import MasterThesis.LOOP.Language
+import MasterThesis.LOOP.Interpreter
 
+namespace SCORE
+
+open SCORE.com
+
+def LOOP2SCORE (Lc : LOOP.com) : SCORE.com :=
+  match Lc with
+  | LOOP.com.SKIP    => SKIP
+  | LOOP.com.ZER x   => CON x
+  | LOOP.com.ASN x y => CON x ;;
+                        FOR y (INC x)
+  | LOOP.com.INC x   => INC x
+  | LOOP.com.SEQ P Q => LOOP2SCORE P ;;
+                        LOOP2SCORE Q
+
+  | LOOP.com.FOR x P => FOR x (LOOP2SCORE P)
+
+namespace LOOP2SCORE
+
+def eqStores (σ : LOOP.store) (τ : SCORE.store) : Prop :=
+  ∀ (x : ident), σ x = (τ x).head!
+
+infix:100 "=ₛ" => eqStores
+
+theorem soundness : ∀ (Lc : LOOP.com) (σ : LOOP.store) (τ : SCORE.store), σ =ₛ τ → (LOOP.eval Lc σ) =ₛ (SCORE.eval (LOOP2SCORE Lc) τ) :=
+  sorry
+
+end LOOP2SCORE
+
+end SCORE
